Some reasoning about reachability

examples/data_structures/graph/Graph.Search.fst
@@ -120,5 +120,138 @@ let rec lemma_bfs_map_pairing_aux (#n:nat) (g:graph0 n{no_parallel_edge g}) (see
     MC.lemma_fold_upd2 parents adj_unscene (fun _ -> hd);
     MC.domain_lemma parents adj_unscene (fun _ -> hd);
 
-    SEC.as_set_mem_in_forall adj_unscene;
+    SEC.as_set_mem_in_forall adj_unscene;    
     lemma_bfs_map_pairing_aux g s' f' p'
+
+
+let rec lemma_bfs_map_ordering_aux (#n:nat) (g:graph0 n{no_parallel_edge g}) (seen:nodeset n) (frntr:nodeset n) (parents:M.t (fin n) (fin n))
+ : Lemma
+   (requires
+     N.disjoint seen frntr /\
+     (forall (x:fin n).  M.contains parents x ==>  (exists (y:fin n) . M.sel parents x == y /\ L.mem y seen)))
+
+   (ensures N.disjoint seen frntr /\
+     (let s', p' = bfs_map_aux g seen frntr parents in
+      (forall (x:fin n).  M.contains parents x ==>  (exists (y:fin n). M.sel p' x == y /\ L.mem y s'))))
+   (decreases (decrease_clause n seen))
+= match frntr with
+  | [] -> ()
+  | hd :: tl ->
+    let adj = g @^ hd in
+    let neither_in_s_nor_f = neither_in seen frntr in
+    let adj_unscene = L.filter neither_in_s_nor_f adj <: list (fin n) in
+    LC.noRepeats_filter neither_in_s_nor_f adj;
+    
+    let s' = hd :: seen in
+    let f' = N.append tl adj_unscene in
+    let p' = fill_map parents adj_unscene hd in
+
+    N.lemma_disjoint_append tl adj_unscene s';
+    LC.filter_sublist neither_in_s_nor_f adj;
+    L.append_mem_forall tl adj_unscene;
+    
+    fill_map_eq_lemma parents adj_unscene hd;
+    MC.lemma_fold_upd1 parents adj_unscene (fun _ -> hd);
+    MC.lemma_fold_upd2 parents adj_unscene (fun _ -> hd);
+    MC.domain_lemma parents adj_unscene (fun _ -> hd);
+    
+    SEC.as_set_mem_in_forall adj_unscene;
+    lemma_bfs_map_ordering_aux g s' f' p'
+
+let adj_implies_reachable (#n:nat) (g:graph0 n) (node:fin n)
+ : Lemma (requires True)
+   (ensures (forall (x:fin n) . L.mem x (g @^ node) ==>  reachable g node x))
+   =
+   let reachable_aux (l:list (fin n))
+       (w:squash(l == g @^ node)) (x:fin n)
+       : Lemma (L.mem x l ==> reachable g node x) =
+       FStar.Squash.give_proof w ;
+       match L.mem x l with
+       | false -> admit()
+       |true ->
+       let p = S.cons node (S.cons x (S.createEmpty)) in 
+       assert(is_in_graph node x g);
+       assert(valid_path g p);
+       assert(from #n #g p == node)
+     in
+     C.forall_intro (reachable_aux (g @^ node)
+    (FStar.Squash.get_proof (g @^ node == g @^ node)))
+
+let adj_reachable (#n:nat) (g:graph0 n) (node:fin n)
+ : Lemma (requires True)
+   (ensures (forall (x:fin n) . L.mem x (g @^ node) ==>  reachable g node x))
+   =
+   let reachable_aux (l:list (fin n))
+       (w:squash(l == g @^ node)) (x:fin n)
+       : Lemma (L.mem x l ==> reachable g node x) =
+       FStar.Squash.give_proof w ;
+       match L.mem x l with
+       | false -> admit()
+       |true ->
+       let p = S.cons node (S.cons x (S.createEmpty)) in 
+       assert(is_in_graph node x g);
+       assert(valid_path g p);
+       assert(from #n #g p == node)
+     in
+     C.forall_intro (reachable_aux (g @^ node)
+    (FStar.Squash.get_proof (g @^ node == g @^ node)))
+
+
+let rec lemma_bfs_reachability (#n:nat) (g:graph0 n{no_parallel_edge g}) (seen:nodeset n) (frntr:nodeset n) (parents:M.t (fin n) (fin n)) (start:fin n)
+ : Lemma (requires
+     N.disjoint seen frntr /\
+     (forall (x: fin n) . L.mem x seen || L.mem x frntr ==>  reachable g start x))
+
+   (ensures N.disjoint seen frntr /\
+     (let s', p' = bfs_map_aux g seen frntr parents in
+      (forall (x:fin n) . L.mem x s' ==>  reachable g start x)))
+   (decreases (decrease_clause n seen))
+  = match frntr with
+  | [] -> ()
+  | hd :: tl ->
+    let adj = g @^ hd in
+    let neither_in_s_nor_f = neither_in seen frntr in
+    let adj_unscene = L.filter neither_in_s_nor_f adj in
+    LC.noRepeats_filter neither_in_s_nor_f adj;
+
+    let s' = hd :: seen in
+    let f' = N.append tl adj_unscene in
+    let p' = fill_map parents adj_unscene hd in
+
+    N.lemma_disjoint_append tl adj_unscene s';
+    LC.filter_sublist neither_in_s_nor_f adj;
+    L.append_mem_forall tl adj_unscene;
+    
+    fill_map_eq_lemma parents adj_unscene hd;
+    MC.lemma_fold_upd1 parents adj_unscene (fun _ -> hd);
+    MC.lemma_fold_upd2 parents adj_unscene (fun _ -> hd);
+    MC.domain_lemma parents adj_unscene (fun _ -> hd);
+
+    SEC.as_set_mem_in_forall adj_unscene;
+
+
+    assume((exists (y:fin n). M.sel p' hd == y /\ L.mem y s'));
+    (*C.exists_elim (reachable g start hd) (FStar.Squash.get_proof (exists (y:fin n). M.sel p' hd == y /\ L.mem y s')) (fun x -> admit());*)
+    (*assume(forall (x:fin n). L.mem x adj_unscene ==> reachable g start x);*)
+    adj_implies_reachable g hd;
+    assert(forall (x:fin n). L.mem x adj_unscene ==> reachable g hd x);
+    let reachable_aux (l:list (fin n))
+       (w:squash(l == adj_unscene)) (x:fin n)
+       : Lemma (L.mem x adj_unscene ==> reachable g start x) =
+       FStar.Squash.give_proof w ;
+           match L.mem x l with
+           | false -> ()
+           |true ->
+           assume((exists (y:fin n). M.sel p' hd == y /\ L.mem y s'));
+           adj_implies_reachable g hd;
+           assert(forall (x:fin n). L.mem x l ==> reachable g hd x);
+           assert(reachable g hd x);
+           C.exists_elim (reachable g start x) (FStar.Squash.get_proof (exists (y:fin n). M.sel p' hd 
+           == y /\ L.mem y s')) (fun e -> lemma_reachable_trans g start hd x); admit()
+     in
+     C.forall_intro (reachable_aux adj_unscene
+    (FStar.Squash.get_proof (adj_unscene == adj_unscene)));
+
+    lemma_bfs_reachability g s' f' p' start
+
+(*(*(forall (e:fin n) . L.mem e l ==> L.mem e adj) /\*) 
